start of datatypes

coq-DataRF/BasicDefinitions.v
@@ -1,8 +1,19 @@
 Require Import Nat.
+Require Import Lists.List.
 
 Definition index := nat.
 Definition vname := nat. (* can change this atoms later *)
 Definition id    := nat.
+Definition Arity := nat.
+
+Record dcons := DCons {
+    dcid    : id;
+    arity   : Arity
+}.
+
+Record tcons := TCons {
+    tcid    : id
+}.
 
 Inductive prim : Set :=
     | And 
@@ -19,7 +30,7 @@ Inductive prim : Set :=
 
 Inductive basic : Set :=
     | TBool 
-    | TInt  
+    | TInt                          
     | BTV   (i : index)
     | FTV   (a : vname).
 
@@ -36,6 +47,7 @@ Inductive basic : Set :=
         | _       => False
         end.  
 
+
 (* ONLY types with Base kind may have non-trivial refinements. Star kinded type variables 
      may only have the refinement { x : [] }. *)
 Inductive kind : Set := 
@@ -46,6 +58,7 @@ Inductive expr : Set :=
     | Bc (b : bool)                 (* True, False *)
     | Ic (n : nat)                  (* 0, 1, 2, *)
     | Prim (p : prim)               (* built-in primitive functions *)
+    | Dc (d : dcons)
     | BV (i : index)                (* BOUND Variables: bound to a Lambda, Let or :t *)
     | FV (x : vname)                (* FREE Variables: bound in an environment *)
     | Lambda (e : expr)             (* \x.e          abstractions    (x is nameless) *)
@@ -54,9 +67,15 @@ Inductive expr : Set :=
     | AppT (e : expr) (t : type)    (* e [bt]   type applications *)
     | Let (e1 : expr) (e2 : expr)   (* let x = e1 in e2              (x is nameless) *)
     | Annot (e : expr) (t : type)   (* e : t *)
+    | Switch (e : expr) (cs : alts)
+
+with alts : Set :=
+    | AEmpty
+    | ACons  (d : dcons) (e : expr) (cs : alts)
 
 with type : Set :=
     | TRefn   (b : basic) (ps : preds)   (* b{x0 : [p]} *)
+    | TData   (tc: tcons) (t:type)  (ps: preds)  (* TODO: is this WLOG? *)
     | TFunc   (tx : type) (t : type)     (* x:t_x -> t *)
     | TExists (tx : type) (t : type)     (* \exists x:t_x. t *)
     | TPoly   (k : kind)  (t : type)     (* \forall a:k. t *)
@@ -66,9 +85,11 @@ with preds : Set :=               (* i.e. [expr] *)
     | PCons (p : expr) (ps : preds).
 
 Scheme expr_mutind  := Induction for expr  Sort Set
+with   alts_mutind  := Induction for alts  Sort Set
 with   type_mutind  := Induction for type  Sort Set
 with   preds_mutind := Induction for preds Sort Set.
-Combined Scheme syntax_mutind from expr_mutind, type_mutind, preds_mutind.
+Combined Scheme syntax_mutind from 
+    expr_mutind, alts_mutind, type_mutind, preds_mutind.
 
     Definition isTRefn (t : type) : Prop  := 
         match t with
@@ -94,48 +115,135 @@ Combined Scheme syntax_mutind from expr_mutind, type_mutind, preds_mutind.
         | _           => False
         end.  
 
-Definition isValue (e: expr) : Prop :=
-    match e with
-    | Bc _          => True
-    | Ic _          => True
-    | Prim c        => True
-    | FV _          => True
-    | BV _          => True
-    | Lambda   _    => True
-    | LambdaT   k e => True
-    | _             => False         
+Inductive isValue : expr -> Set := (* can't use Prop here *)
+    | val_Bc   : forall b,   isValue (Bc b)
+    | val_Ic   : forall n,   isValue (Ic n)
+    | val_Prm  : forall c,   isValue (Prim c)
+    | val_BV   : forall i,   isValue (BV i)
+    | val_FV   : forall x,   isValue (FV x)
+    | val_Lam  : forall e,   isValue (Lambda e)
+    | val_LamT : forall k e, isValue (LambdaT k e)
+    | val_dv   : forall dv,  dataValue dv -> isValue dv
+
+with dataValue : expr -> Set :=
+    | dval_Dc  : forall dc,   dataValue (Dc dc)
+    | dval_App : forall dv v, dataValue dv -> isValue v -> dataValue (App dv v).
+
+Fixpoint dvdc (dv : expr) (pf : dataValue dv) : dcons :=
+    match pf with
+    | dval_Dc  dc               => dc
+    | dval_App dv v dv_pf v_pf  => dvdc dv dv_pf
     end.
 
-Definition value := { v:expr | isValue v }.
-Definition toExpr (v0 : value) : expr :=
-    match v0 with 
-    | exist _ e _ => e
+Fixpoint argCount (dv: expr) (pf : dataValue dv) : nat :=
+    match pf with
+    | dval_Dc  dc               => 0
+    | dval_App dv v dv_pf v_pf  => S (argCount dv dv_pf)
     end.
+
+Fixpoint dvdc' (dv : expr) : option dcons :=
+    match dv with
+    | Dc dc     => Some dc
+    | App dv v  => dvdc' dv
+    | _         => None
+    end.
+
+Fixpoint argCount' (dv : expr) : option nat :=
+    match dv with
+    | Dc _     => Some 0
+    | App dv v => option_map S (argCount' dv) 
+    | _        => None
+    end.
+
+Lemma dvdc_dvdc' : forall (dv : expr) (pf : dataValue dv),
+    dvdc' dv = Some (dvdc dv pf).
+Proof. intros. induction pf as [dc|dv v Hdv IH Hv]; simpl;
+  try rewrite IH; simpl; reflexivity. Qed.
+
+Lemma dvdc_pf_indep : forall (dv : expr) (pf pf' : dataValue dv),
+    dvdc dv pf = dvdc dv pf'.
+Proof. intros. assert (Some (dvdc dv pf) = Some (dvdc dv pf')).
+- apply eq_stepl with (dvdc' dv); apply dvdc_dvdc'.
+- injection H as H'; assumption. Qed.
+
+Definition fullyApplied (dv: expr) (pf : dataValue dv) : Prop :=
+    argCount dv pf = arity (dvdc dv pf).
 
 Fixpoint noExists (t0 : type) : Prop := 
     match t0 with         
     | (TRefn b ps)     => True  
+    | (TData tc t ps)  => noExists t
     | (TFunc  t_x t)   => noExists t_x /\ noExists t
     | (TExists  t_x t) => False
     | (TPoly  k   t)   => noExists t
     end.
-(* This would also avoid issues of deBruijn index shifting 
---   in type variable substitution (in defining push) *)
-Definition usertype := { t:type | noExists t }.
-Definition toType (ut : usertype) : type :=
-    match ut with
-    | exist _ t _ => t
+
+    (* This would also avoid issues of deBruijn index shifting 
+    --   in type variable substitution (in defining push) *)
+    Definition usertype := { t:type | noExists t }.
+    Definition toType (ut : usertype) : type :=
+        match ut with
+        | exist _ t _ => t
+        end.
+
+    Lemma texists_not_usertype : forall (t_x t : type),
+        noExists (TExists t_x t) -> False.
+    Proof. simpl. contradiction. Qed.
+
+Fixpoint arrows (t:type) : nat := 
+    match t with 
+    | (TFunc t_x t)  => 1 + (arrows t)
+    | _              => 0
     end.
 
-Lemma texists_not_usertype : forall (t_x t : type),
-    noExists (TExists t_x t) -> False.
-Proof. simpl. contradiction. Qed.
+Definition quant_arrows (t : type) : nat := 
+    match t with 
+    | (TPoly k t) => arrows t
+    | _           => 0
+    end.
+
+  (* --- DEFINITIONAL ENVIRONMENTS ---  
+      -- not currently enforced: but we assume that every
+      --     DCons id is globally unique *)
+
+Record ddefn := DDefn {
+    dddc    : dcons;
+    ddtype  : type
+}.
+
+Inductive polarity : Set := 
+    | Pos 
+    | Neg 
+    | Both 
+    | Neither.
+
+Inductive ddefns : Set :=  
+    | DDEmpty 
+    | DDCons (dd : ddefn) (dds : ddefns).
+
+Record tdefn := TDefn { 
+    tdid     : id;
+    vkind    : kind;
+    vpolar   : polarity;
+    tddcons  : ddefns 
+}.        
+
+Definition defs := list tdefn.
+
+Fixpoint tcKind (tc : tcons) (tds : defs) : option kind :=
+    match tds with
+    | nil          => None
+    | (td :: tds)  => if tcid tc =? tdid td then Some (vkind td)  
+                                            else tcKind tc tds
+    end.
+
 
 Fixpoint isLC_at (j_x : index) (j_a : index) (e : expr) : Prop  :=
     match e with
     | (Bc _)         => True
     | (Ic _)         => True
     | (Prim _)       => True
+    | (Dc _)         => True
     | (BV i)         => i < j_x
     | (FV _)         => True
     | (Lambda e')    => isLC_at (j_x + 1) j_a e'
@@ -144,14 +252,23 @@ Fixpoint isLC_at (j_x : index) (j_a : index) (e : expr) : Prop  :=
     | (AppT e' t)    => isLC_at j_x j_a e'    /\ isLCT_at j_x j_a t 
     | (Let ex e')    => isLC_at j_x j_a ex    /\ isLC_at (j_x+1) j_a e'  
     | (Annot e' t)   => isLC_at j_x j_a e'    /\ isLCT_at j_x j_a t 
+    | (Switch e cs)  => isLC_at j_x j_a e     /\ isLCA_at j_x j_a cs
+    end
+
+with isLCA_at (j_x : index) (j_a : index) (cs : alts) : Prop :=
+    match cs with 
+    | AEmpty          => True
+    | (ACons dc e cs) => isLC_at (j_x + (arity dc)) j_a e /\ isLCA_at j_x j_a cs
     end
 
 with isLCT_at (j_x : index) (j_a : index) (t0 : type) : Prop := 
     match t0 with
-    | (TRefn   b  rs) =>  match b with
-                          | (BTV i) => i < j_a /\ isLCP_at (j_x+1) j_a rs
-                          | _       =>            isLCP_at (j_x+1) j_a rs
-                          end
+    | (TRefn   b  rs) =>  
+          match b with          
+          | (BTV i) => i < j_a /\ isLCP_at (j_x+1) j_a rs
+          | _       =>            isLCP_at (j_x+1) j_a rs
+          end
+    | (TData tc t ps) => isLCT_at j_x j_a t /\ isLCP_at (j_x+1) j_a ps
     | (TFunc   t_x t) => isLCT_at j_x j_a t_x /\ isLCT_at (j_x+1) j_a t
     | (TExists t_x t) => isLCT_at j_x j_a t_x /\ isLCT_at (j_x+1) j_a t
     | (TPoly   k   t) =>                         isLCT_at j_x (j_a+1) t
@@ -164,6 +281,7 @@ with isLCP_at (j_x : index) (j_a : index) (ps0 : preds) : Prop :=
     end.
 
 Definition isLC  (e  : expr)  : Prop := isLC_at  0 0 e.
+Definition isLCA (cs : alts)  : Prop := isLCA_at 0 0 cs.
 Definition isLCT (t  : type)  : Prop := isLCT_at 0 0 t.
 Definition isLCP (ps : preds) : Prop := isLCP_at 0 0 ps.
 
@@ -172,6 +290,7 @@ Fixpoint open_at (j : index) (y : vname) (e : expr) : expr :=
     | (Bc b)             => Bc b
     | (Ic n)             => Ic n
     | (Prim c)           => Prim c
+    | (Dc dc)            => Dc dc
     | (BV i)             => if j =? i then FV y else BV i 
     | (FV x)             => FV x
     | (Lambda e')        => Lambda (open_at (j+1) y e')
@@ -180,11 +299,19 @@ Fixpoint open_at (j : index) (y : vname) (e : expr) : expr :=
     | (AppT e' t)        => AppT  (open_at j y e')  (openT_at j y t)
     | (Let ex e')        => Let   (open_at j y ex) (open_at (j+1) y e')
     | (Annot e' t)       => Annot (open_at j y e')  (openT_at j y t)
+    | (Switch e cs)      => Switch (open_at j y e)  (openA_at j y cs)
+    end
+
+with openA_at (j : index) (y : vname) (cs : alts) : alts :=
+    match cs with
+    | AEmpty          => AEmpty
+    | (ACons dc e cs) => ACons dc (open_at (j + (arity dc)) y e) (openA_at j y cs)
     end
 
 with openT_at (j : index) (y : vname) (t0 : type) : type :=
     match t0 with
-    | (TRefn b ps)    => TRefn b (openP_at (j+1) y ps)
+    | (TRefn b ps)    => TRefn b                    (openP_at (j+1) y ps)
+    | (TData tc t ps) => TData tc (openT_at j y t)  (openP_at (j+1) y ps)
     | (TFunc   t_z t) => TFunc   (openT_at j y t_z) (openT_at (j+1) y t)
     | (TExists t_z t) => TExists (openT_at j y t_z) (openT_at (j+1) y t)
     | (TPoly   k   t) => TPoly k (openT_at j y t) 
@@ -197,6 +324,7 @@ with openP_at (j : index) (y : vname) (ps0 : preds) : preds  :=
     end.
 
 Definition unbind  (y : vname) (e : expr)   : expr  :=  open_at 0 y e. 
+Definition unbindA (y : vname) (cs : alts)  : alts  :=  openA_at 0 y cs.
 Definition unbindT (y : vname) (t : type)   : type  :=  openT_at 0 y t.
 Definition unbindP (y : vname) (ps : preds) : preds :=  openP_at 0 y ps.
 
@@ -206,6 +334,7 @@ Fixpoint open_tv_at (j : index) (a' : vname) (e0 : expr) : expr :=
     | (Bc b)                       => Bc b
     | (Ic n)                       => Ic n
     | (Prim p)                     => Prim p
+    | (Dc dc)                      => Dc dc
     | (BV i)                       => BV i    (* looking for type vars *)
     | (FV y)                       => FV y
     | (Lambda e)                   => Lambda    (open_tv_at j a' e)  
@@ -214,15 +343,24 @@ Fixpoint open_tv_at (j : index) (a' : vname) (e0 : expr) : expr :=
     | (AppT e t)                   => AppT      (open_tv_at j a' e)  (open_tvT_at j a' t)
     | (Let e1 e2  )                => Let       (open_tv_at j a' e1) (open_tv_at  j a' e2) 
     | (Annot e t)                  => Annot     (open_tv_at j a' e)  (open_tvT_at j a' t)
+    | (Switch e cs)                => Switch    (open_tv_at j a' e)  (open_tvA_at j a' cs)
+    end
+
+with open_tvA_at (j : index) (a' : vname) (cs : alts) : alts  :=
+    match cs with
+    | AEmpty          => AEmpty
+    | (ACons dc e cs) => ACons dc (open_tv_at j a' e) (open_tvA_at j a' cs)    
     end
 
 with open_tvT_at (j : index) (a' : vname) (t0 : type) : type  :=
     match t0 with
-    | (TRefn b  ps)     => match b with 
+    | (TRefn b  ps)     => 
+          match b with 
           | (BTV i)  => if j =? i then TRefn (FTV a') (open_tvP_at j a' ps) 
                                   else TRefn b        (open_tvP_at j a' ps)
           | _        =>                TRefn b        (open_tvP_at j a' ps) 
           end
+    | (TData tc t ps)   => TData tc (open_tvT_at j a' t)   (open_tvP_at j a' ps)
     | (TFunc   t_z t)   => TFunc    (open_tvT_at j a' t_z) (open_tvT_at j a' t)
     | (TExists t_z t)   => TExists  (open_tvT_at j a' t_z) (open_tvT_at j a' t)
     | (TPoly   k  t)    => TPoly k  (open_tvT_at (j+1) a' t)
@@ -235,6 +373,7 @@ with open_tvP_at (j : index) (a' : vname) (ps0 : preds) : preds  :=
     end.
 
 Definition unbind_tv  (a' : vname) (e : expr) : expr  :=  open_tv_at 0 a' e.
+Definition unbind_tvA (a' : vname) (cs: alts) : alts  :=  open_tvA_at 0 a' cs.
 Definition unbind_tvT (a' : vname) (t : type) : type  :=  open_tvT_at 0 a' t.
 Definition unbind_tvP (a' : vname) (ps : preds) : preds := open_tvP_at 0 a' ps.
 
@@ -245,6 +384,7 @@ Fixpoint shift_at (j k : index) (e : expr) : expr :=
     | (Bc b)             => Bc b
     | (Ic n)             => Ic n
     | (Prim c)           => Prim c
+    | (Dc dc)            => Dc dc
     | (BV i)             => if i <=? j then BV (i+1) else BV i 
     | (FV x)             => FV x
     | (Lambda e')        => Lambda (shift_at (j+1) k e')
@@ -253,11 +393,19 @@ Fixpoint shift_at (j k : index) (e : expr) : expr :=
     | (AppT e' t)        => AppT  (shift_at j k e')  (shiftT_at j k t)
     | (Let ex e')        => Let   (shift_at j k ex)  (shift_at (j+1) k e')
     | (Annot e' t)       => Annot (shift_at j k e')  (shiftT_at j k t)
+    | (Switch e cs)      => Switch (shift_at j k e)  (shiftA_at j k cs)
+    end
+
+with shiftA_at (j k : index) (cs : alts) : alts :=
+    match cs with    
+    | AEmpty        => AEmpty
+    | ACons dc e cs => ACons dc (shift_at j k e) (shiftA_at j k cs)
     end
 
 with shiftT_at (j k : index) (t0 : type) : type :=
     match t0 with
     | (TRefn b ps)    => TRefn b (shiftP_at (j+1) k ps)
+    | (TData tc t ps) => TData tc (shiftT_at j k t)  (shiftP_at (j+1) k ps)  
     | (TFunc   t_z t) => TFunc   (shiftT_at j k t_z) (shiftT_at (j+1) k t)
     | (TExists t_z t) => TExists (shiftT_at j k t_z) (shiftT_at (j+1) k t)
     | (TPoly   k0  t) => TPoly k0 (shiftT_at j (k+1) t) 
@@ -277,6 +425,7 @@ Fixpoint subFV (x : vname) (v_x : expr) (e0 : expr) : expr :=
     | (Bc b)                    => Bc b
     | (Ic n)                    => Ic n
     | (Prim p)                  => Prim p
+    | (Dc dc)                   => Dc dc
     | (BV i)                    => BV i
     | (FV y)                    => if x =? y then v_x else FV y
     | (Lambda   e)              => Lambda    (subFV x v_x e)
@@ -285,11 +434,19 @@ Fixpoint subFV (x : vname) (v_x : expr) (e0 : expr) : expr :=
     | (AppT e bt)               => AppT  (subFV x v_x e) (tsubFV x v_x bt)
     | (Let   e1 e2)             => Let   (subFV x v_x e1) (subFV x v_x e2)
     | (Annot e t)               => Annot (subFV x v_x e) (tsubFV x v_x t) 
+    | (Switch e cs)             => Switch (subFV x v_x e) (asubFV x v_x cs) 
+    end
+
+with asubFV (x : vname) (v_x : expr) (cs : alts) : alts :=
+    match cs with
+    | AEmpty          => AEmpty
+    | (ACons dc e cs) => ACons dc (subFV x v_x e) (asubFV x v_x cs)
     end
 
 with tsubFV (x : vname) (v_x : expr) (t0 : type) : type :=
     match t0 with
     | (TRefn  b r)     => TRefn b   (psubFV x v_x r)
+    | (TData tc t ps)  => TData tc (tsubFV x v_x t)   (psubFV x v_x ps)
     | (TFunc  t_z t)   => TFunc    (tsubFV x v_x t_z) (tsubFV x v_x t)
     | (TExists  t_z t) => TExists  (tsubFV x v_x t_z) (tsubFV x v_x t)
     | (TPoly  k   t)   => TPoly    k                  (tsubFV x v_x t)
@@ -314,6 +471,7 @@ Fixpoint strengthen (qs : preds) (rs : preds) : preds :=
 Fixpoint push (p : preds) (t0 : type) : type := 
     match t0 with
     | (TRefn   b     r)  => TRefn   b     (strengthen p r)
+    | (TData   tc t  r)  => TData   tc t  (strengthen p r)
     | (TFunc     t_y t)  => TFunc     t_y t
     | (TExists   t_y t)  => TExists   t_y (push (shiftP p) t)
         (* wanted: match texists_not_usertype t_y t pf with end *)
@@ -325,6 +483,7 @@ Fixpoint subFTV (a : vname) (t_a : type) (e0 : expr) : expr :=
     | (Bc b)                    => Bc b
     | (Ic n)                    => Ic n
     | (Prim p)                  => Prim p
+    | (Dc dc)                   => Dc dc
     | (BV i)                    => BV i
     | (FV y)                    => FV y
     | (Lambda   e)              => Lambda     (subFTV a t_a e)
@@ -333,15 +492,23 @@ Fixpoint subFTV (a : vname) (t_a : type) (e0 : expr) : expr :=
     | (AppT e t)                => AppT  (subFTV a t_a e) (tsubFTV a t_a t)
     | (Let   e1 e2)             => Let   (subFTV a t_a e1) (subFTV a t_a e2)
     | (Annot e t)               => Annot (subFTV a t_a e) (tsubFTV a t_a t) 
+    | (Switch e cs)             => Switch (subFTV a t_a e) (asubFTV a t_a cs) 
+    end
+
+with asubFTV (a : vname) (t_a : type) (cs : alts) : alts  :=
+    match cs with
+    | AEmpty          => AEmpty
+    | (ACons dc e cs) => ACons dc (subFTV a t_a e) (asubFTV a t_a cs)
     end
 
 with tsubFTV (a : vname) (t_a : type) (t0 : type) : type  :=
     match t0 with
-    | (TRefn b   r)        => match b with
+    | (TRefn b   r)        => match b with         
           | (FTV a')   => if a =? a' then push      (psubFTV a t_a r) t_a
                                      else TRefn b   (psubFTV a t_a r)
           | _          =>                 TRefn b   (psubFTV a t_a r)
           end
+    | (TData tc t r)       => TData tc (tsubFTV a t_a t)     (psubFTV a t_a r)       
     | (TFunc     t_z t)    => TFunc      (tsubFTV a t_a t_z) (tsubFTV a t_a t)
     | (TExists   t_z t)    => TExists    (tsubFTV a t_a t_z) (tsubFTV a t_a t)
     | (TPoly      k  t)    => TPoly      k                   (tsubFTV a t_a t)
@@ -358,6 +525,7 @@ Fixpoint subBV_at (j : index) (v : expr) (e0 : expr) : expr :=
     | (Bc b)             => Bc b
     | (Ic n)             => Ic n
     | (Prim c)           => Prim c
+    | (Dc dc)            => Dc dc
     | (BV i)             => if j =? i then v else BV i
     | (FV x)             => FV x
     | (Lambda e)         => Lambda (subBV_at (j+1) v e)
@@ -366,11 +534,19 @@ Fixpoint subBV_at (j : index) (v : expr) (e0 : expr) : expr :=
     | (AppT e t)         => AppT  (subBV_at j v e)  (tsubBV_at j v t)
     | (Let ex e)         => Let   (subBV_at j v ex) (subBV_at (j+1) v e)
     | (Annot e t)        => Annot (subBV_at j v e)  (tsubBV_at j v t)
+    | (Switch e cs)      => Switch (subBV_at j v e)  (asubBV_at j v cs)
+    end
+
+with asubBV_at (j : index) (v_x : expr) (cs : alts) : alts :=
+    match cs with
+    | AEmpty          => AEmpty
+    | (ACons dc e cs) => ACons dc (subBV_at (j+(arity dc)) v_x e) (asubBV_at j v_x cs)
     end
 
 with tsubBV_at (j : index) (v_x : expr) (t0 : type) : type :=
     match t0 with
     | (TRefn b ps)    => TRefn b (psubBV_at (j+1) v_x ps)  
+    | (TData tc t ps) => TData tc (tsubBV_at j v_x t)  (psubBV_at (j+1) v_x ps)  
     | (TFunc   t_z t) => TFunc   (tsubBV_at j v_x t_z) (tsubBV_at (j+1) v_x t)
     | (TExists t_z t) => TExists (tsubBV_at j v_x t_z) (tsubBV_at (j+1) v_x t)
     | (TPoly   k  t)  => TPoly k (tsubBV_at j v_x t)  
@@ -383,6 +559,7 @@ with psubBV_at (j : index) (v_x : expr) (ps0 : preds) : preds  :=
     end.
 
 Definition subBV  (v : expr) (e : expr)   : expr  :=  subBV_at 0 v e.
+Definition asubBV (v_x : expr) (cs: alts) : alts  :=  asubBV_at 0 v_x cs.
 Definition tsubBV (v_x : expr) (t : type) : type  :=  tsubBV_at 0 v_x t.
 Definition psubBV (v : expr) (ps : preds) : preds :=  psubBV_at 0 v ps.
 
@@ -391,6 +568,7 @@ Fixpoint subBTV_at (j : index) (t_a : type) (e0 : expr) : expr :=
     | (Bc b)                       => Bc b
     | (Ic n)                       => Ic n
     | (Prim p)                     => Prim p
+    | (Dc dc)                      => Dc dc
     | (BV i)                       => BV i 
     | (FV y)                       => FV y
     | (Lambda   e)                 => Lambda    (subBTV_at j t_a e)  
@@ -399,15 +577,24 @@ Fixpoint subBTV_at (j : index) (t_a : type) (e0 : expr) : expr :=
     | (AppT e t)                   => AppT      (subBTV_at j t_a e) (tsubBTV_at j t_a t)
     | (Let   e1 e2)                => Let       (subBTV_at j t_a e1) (subBTV_at j t_a e2) 
     | (Annot e t)                  => Annot     (subBTV_at j t_a e) (tsubBTV_at j t_a t)
+    | (Switch e cs)                => Switch    (subBTV_at j t_a e) (asubBTV_at j t_a cs)
+    end
+
+with asubBTV_at (j : index) (t_a : type) (cs : alts) : alts :=
+    match cs with
+    | AEmpty          => AEmpty
+    | (ACons dc e cs) => ACons dc (subBTV_at j t_a e) (asubBTV_at j t_a cs)
     end
 
 with tsubBTV_at (j : index) (t_a : type) (t0 : type) : type :=
     match t0 with
-    | (TRefn b   ps)     => match b with
+    | (TRefn b   ps)     => 
+          match b with
           | (BTV i) => if j =? i then push (psubBTV_at j t_a ps) t_a 
                                  else TRefn b (psubBTV_at j t_a ps) (* TExists y t_y (push x r[t_a/a] t')  *)
           | _       =>                TRefn b (psubBTV_at j t_a ps)    
           end
+    | (TData tc t ps)    => TData tc (tsubBTV_at j t_a t)   (psubBTV_at j t_a ps)
     | (TFunc   t_z t)    => TFunc    (tsubBTV_at j t_a t_z) (tsubBTV_at j t_a t)  
     | (TExists t_z t)    => TExists  (tsubBTV_at j t_a t_z) (tsubBTV_at j t_a t)  
     | (TPoly   k  t)     => TPoly k  (tsubBTV_at (j+1) t_a t)
@@ -420,6 +607,7 @@ with psubBTV_at (j : index) (t_a : type) (ps0 : preds) : preds :=
     end.
 
 Definition subBTV  (t : type)   (e : expr)   : expr  :=  subBTV_at 0 t e.
+Definition asubBTV (t_a : type) (cs : alts)  : alts  :=  asubBTV_at 0 t_a cs.
 Definition tsubBTV (t_a : type) (t : type)   : type  :=  tsubBTV_at 0 t_a t.
 Definition psubBTV (t_a : type) (ps : preds) : preds :=  psubBTV_at 0 t_a ps.
 
@@ -429,6 +617,7 @@ Definition psubBTV (t_a : type) (ps : preds) : preds :=  psubBTV_at 0 t_a ps.
 
 Inductive ftype : Set :=
     | FTBasic (b : basic)                (* b: Bool, Int, FTV a, BTV a *)
+    | FTData  (tc : tcons) (t : ftype)
     | FTFunc  (t1 : ftype) (t2 : ftype)  (* bt -> bt' *)
     | FTPoly  (k : kind) (t : ftype).    (* \forall a:k. bt *)
 
@@ -444,10 +633,29 @@ Inductive ftype : Set :=
         | (FTBasic TInt)  => True
         | _               => False
         end.
+    
+    Definition isFTData (t : ftype) : Prop :=
+        match t with
+        | (FTData _ _) => True
+        | _            => False
+        end.
+
+Fixpoint arrowsF (t:ftype) : nat := 
+    match t with 
+    | (FTFunc t_x t)  => 1 + (arrowsF t)
+    | _               => 0
+    end.
+
+Definition quant_arrowsF (t : ftype) : nat := 
+    match t with 
+    | (FTPoly k t) => arrowsF t
+    | _            => 0
+    end.
 
 Fixpoint erase (t0 : type) : ftype :=
     match t0 with
     | (TRefn b r)     => FTBasic b
+    | (TData tc t r)  => FTData tc (erase t)
     | (TFunc t_x t)   => FTFunc (erase t_x) (erase t)
     | (TExists t_x t) => (erase t)
     | (TPoly  k  t)   => FTPoly k (erase t)
@@ -459,6 +667,7 @@ Fixpoint isLCFT_at (j : index) (t0 : ftype) : Prop :=
                           | (BTV i)   => i < j
                           | _         => True
                           end
+    | (FTData tc t)    => isLCFT_at j t
     | (FTFunc t_x t)   => isLCFT_at j t_x /\ isLCFT_at j t
     | (FTPoly   k t)   => isLCFT_at (j+1) t
     end.
@@ -471,6 +680,7 @@ Fixpoint openFT_at (j : index) (a' : vname) (t0 : ftype) : ftype :=
                         | (BTV i) => if j =? i then FTBasic (FTV a') else FTBasic b
                         | _       => FTBasic b
                         end
+    | (FTData tc  t) => FTData tc (openFT_at j a' t)
     | (FTFunc t_x t) => FTFunc (openFT_at j a' t_x) (openFT_at j a' t)
     | (FTPoly k   t) => FTPoly k (openFT_at (j+1) a' t)
     end.
@@ -483,6 +693,7 @@ Fixpoint ftsubFV (a : vname) (t_a : ftype) (t0 : ftype) : ftype :=
                          | (FTV a')  => if a =? a' then t_a else FTBasic b
                          | _         => FTBasic b
                          end
+    | (FTData tc  t)  => FTData tc (ftsubFV a t_a t)
     | (FTFunc t_z t)  => FTFunc (ftsubFV a t_a t_z) (ftsubFV a t_a t)
     | (FTPoly   k t)  => FTPoly k (ftsubFV a t_a t)
     end.
@@ -493,6 +704,7 @@ Fixpoint ftsubBV_at (j : index) (t_a : ftype) (t0 : ftype) : ftype :=
                           | (BTV i) => if j =? i then t_a else FTBasic b
                           | _       => FTBasic b
                           end
+    | (FTData tc  t)  => FTData tc (ftsubBV_at j t_a t)
     | (FTFunc t_z t)  => FTFunc (ftsubBV_at j t_a t_z) (ftsubBV_at j t_a t)
     | (FTPoly  k  t)  => FTPoly k (ftsubBV_at (j+1) t_a t)
     end.
